src/matroid/submatroids/matroid_in.lean
@@ -21,8 +21,7 @@ variables {E α : Type*} [finite E] [finite α]
   -/
 
 /-- A matroid on some subset `E` of `α`. Implemented as a `matroid` in which the elements 
-outside `E` are all loops. The matroid `carrier` is a detail of this implentation, and not 
-intended to be accessed directly.  -/
+outside `E` are all loops. -/
 @[ext] structure matroid_in (α : Type*) [finite α] :=
 (E : set α)
 (carrier : matroid α)
@@ -30,181 +29,303 @@ intended to be accessed directly.  -/
 
 namespace matroid_in
 
+instance {α : Type*} [finite α] : has_coe (matroid_in α) (matroid α) := ⟨λ M, M.carrier⟩ 
+
+@[simp] lemma carrier_eq_coe {M : matroid_in α} : M.carrier = (M : matroid α) := rfl  
+
 section defs
 /- Definitions -/
 
 variables (M : matroid_in α)
 
-def base (B : set α) : Prop :=
-  M.carrier.base B
+def base (B : set α) : Prop := (M : matroid α).base B
 
-def indep (I : set α) : Prop :=
-  ∃ B, M.base B ∧ I ⊆ B
+def indep (I : set α) : Prop := (M : matroid α).indep I 
+  -- ∃ B, M.base B ∧ I ⊆ B
 
-def basis (I X : set α) : Prop :=
-  M.indep I ∧ I ⊆ X ∧ ∀ J, M.indep J → I ⊆ J → J ⊆ X → I = J
+def basis (I X : set α) : Prop := (M : matroid α).basis I X 
+  -- M.indep I ∧ I ⊆ X ∧ ∀ J, M.indep J → I ⊆ J → J ⊆ X → I = J
 
-def circuit (C : set α) : Prop :=
-  ¬M.indep C ∧ ∀ I ⊂ C, M.indep I
+def circuit (C : set α) : Prop := (M : matroid α).circuit C ∧ C ⊆ M.E  
+  -- ¬M.indep C ∧ ∀ I ⊂ C, M.indep I
 
-def r (X : set α) : ℕ :=
-  M.carrier.r X
+def r (X : set α) : ℕ := (M : matroid α).r X 
+  -- M.carrier.r X
 
-def flat (F : set α) : Prop := 
-  F ⊆ M.E ∧ ∀ I X, M.basis I F → M.basis I X → X ⊆ F 
+def flat (F : set α) : Prop := (M : matroid α).flat (F ∪ M.Eᶜ) ∧ F ⊆ M.E  
+  -- F ⊆ M.E ∧ ∀ I X, M.basis I F → M.basis I X → X ⊆ F 
 
-def cl (X : set α) : set α :=
-  ⋂₀ {F | M.flat F ∧ X ⊆ F}
+def cl (X : set α) : set α := (M : matroid α).cl X ∩ M.E 
+  -- ⋂₀ {F | M.flat F ∧ X ⊆ F}
 
-def hyperplane (H : set α) : Prop :=
-  M.flat H ∧ H ⊂ M.E ∧ (∀ F, H ⊂ F → M.flat F → F = M.E)
+def hyperplane (H : set α) : Prop := (M : matroid α).hyperplane (H ∪ M.Eᶜ) ∧ H ⊆ M.E  
+  -- M.flat H ∧ H ⊂ M.E ∧ (∀ F, H ⊂ F → M.flat F → F = M.E)
 
-def loop (e : α) : Prop :=
-  M.circuit {e}
+def loop (e : α) : Prop := (M : matroid α).loop e ∧ e ∈ M.E  
+  -- M.circuit {e}
 
-def coloop (e : α) : Prop :=
-  ∀ B, M.base B → e ∈ B
+def nonloop (e : α) : Prop := (M : matroid α).nonloop e 
 
-def cocircuit (K : set α) : Prop :=
-  M.hyperplane (M.E \ K)
+def coloop (e : α) : Prop := (M : matroid α).coloop e 
+  -- ∀ B, M.base B → e ∈ B
+
+def cocircuit (K : set α) : Prop := (M : matroid α).cocircuit K 
+  -- M.hyperplane (M.E \ K)
 
 end defs
 
-variables {M₁ M₂ M : matroid_in α} {X Y I B C : set α} {e f x y : α}
+section basic 
 
-section carrier
+variables {M : matroid_in α} {X Y I C B F H K : set α} {e f : α}
 
-/- The lemmas in this section break the abstraction between `M` and its `carrier`, and are only
-  used for basic API setup. -/
+lemma loop_coe_of_not_mem_ground (h : e ∉ M.E) : (M : matroid α).loop e := M.support (mem_compl h)
 
-lemma subset_ground_of_disjoint_loops (hX : disjoint X (M.carrier.cl ∅)) : 
-  X ⊆ M.E :=
+lemma mem_ground_of_nonloop_coe (h : (M : matroid α).nonloop e) : e ∈ M.E := 
+by_contra (λ he, h (M.support he))
+
+lemma compl_ground_subset_loops_coe (M : matroid_in α) : M.Eᶜ ⊆ (M : matroid α).cl ∅ := M.support
+
+lemma subset_ground_of_disjoint_loops_coe (hX : disjoint X ((M : matroid α).cl ∅)) : X ⊆ M.E :=
 (subset_compl_iff_disjoint_right.mpr hX).trans (compl_subset_comm.mp M.support) 
 
-lemma mem_ground_of_nonloop (he : ¬M.carrier.loop e) : 
-  e ∈ M.E :=
+lemma indep.subset_ground (hI : M.indep I) : I ⊆ M.E := 
+  subset_ground_of_disjoint_loops_coe (matroid.indep.disjoint_loops hI)
+
+lemma base_iff_coe : M.base B ↔ (M : matroid α).base B := iff.rfl 
+
+lemma exists_base (M : matroid_in α) : ∃ B, M.base B := matroid.exists_base M  
+
+lemma base.indep (hB : M.base B) : M.indep B := matroid.base.indep hB
+
+lemma base.subset_ground (hB : M.base B) : B ⊆ M.E := hB.indep.subset_ground 
+
+lemma indep_iff_coe : M.indep I ↔ (M : matroid α).indep I := iff.rfl 
+
+lemma indep_iff_subset_base : M.indep I ↔ ∃ B, M.base B ∧ I ⊆ B := iff.rfl   
+
+lemma indep.subset (hI : M.indep I) (hX : X ⊆ I) : M.indep X := matroid.indep.subset hI hX 
+
+lemma indep.r (hI : M.indep I) : M.r I = I.ncard := matroid.indep.r hI
+
+lemma indep.subset_basis_of_subset (hI : M.indep I) (hIX : I ⊆ X) : ∃ J, I ⊆ J ∧ M.basis J X :=
+matroid.indep.subset_basis_of_subset hI hIX   
+
+lemma circuit.subset_ground (hC : M.circuit C) : C ⊆ M.E := hC.2 
+
+lemma circuit_iff : M.circuit C ↔ (¬ M.indep C ∧ (∀ I ⊂ C, M.indep I)) ∧ C ⊆ M.E := 
+⟨λ h, ⟨h.1, h.subset_ground⟩, id⟩
+
+lemma basis_iff_coe : M.basis I X ↔ (M : matroid α).basis I X := iff.rfl 
+
+lemma basis.indep (hIX : M.basis I X) : M.indep I := matroid.basis.indep hIX 
+
+lemma basis.subset (hIX : M.basis I X) : I ⊆ X := matroid.basis.subset hIX 
+
+lemma exists_basis (M : matroid_in α) (X : set α) : ∃ I, M.basis I X := matroid.exists_basis M X
+
+lemma basis.r (hIX : M.basis I X) : M.r I = M.r X := matroid.basis.r hIX
+
+lemma cl_subset_ground (M : matroid_in α) (X : set α) : M.cl X ⊆ M.E := inter_subset_right _ _
+
+lemma subset_cl (hX : X ⊆ M.E) : X ⊆ M.cl X := subset_inter (matroid.subset_cl M X) hX
+
+lemma cl_subset_coe_cl (M : matroid_in α) (X : set α) : M.cl X ⊆ (M : matroid α).cl X := 
+inter_subset_left _ _ 
+
+lemma cl_mono (hXY : X ⊆ Y) (hY : Y ⊆ M.E) : M.cl X ⊆ M.cl Y := 
+subset_inter ((M.cl_subset_coe_cl _).trans (matroid.cl_mono M hXY)) (cl_subset_ground _ _)
+
+@[simp] lemma cl_cl (M : matroid_in α) (X : set α) : M.cl (M.cl X) = M.cl X := 
 begin
-  rw [loop_iff_mem_cl_empty] at he,
-  by_contra h',
-  rw ←mem_compl_iff at h',
-  exact he (M.support h')
-end
-
-lemma subset_ground_of_base_carrier (hB : M.carrier.base B) : 
-  B ⊆ M.E := 
-λ e he, mem_ground_of_nonloop (hB.indep.nonloop_of_mem he)  
-
-lemma subset_ground_of_indep_carrier (hI : M.carrier.indep I) : 
-  I ⊆ M.E :=
-by {obtain ⟨B, hB, hIB⟩ := hI, exact hIB.trans (subset_ground_of_base_carrier hB)}
-
-lemma indep_iff_carrier_indep :
-  M.indep I ↔ M.carrier.indep I :=
-by simp_rw [matroid_in.indep, matroid_in.base, matroid.indep_iff_subset_base]
-
-lemma r_ground_compl (M : matroid_in α) :
-  M.r (M.Eᶜ) = 0 :=
-begin
-  refine r_eq_zero_of_loopy (λ e he, by_contra (λ he', he (mem_ground_of_nonloop _))), 
-  rwa loop_iff_r, 
+  refine (subset_cl (M.cl_subset_ground X)).antisymm' (subset_inter _ (M.cl_subset_ground _)), 
+  refine ((inter_subset_left _ _).trans _), 
+  rw ←matroid.cl_cl (M : matroid α) X, 
+  exact matroid.cl_mono _ (M.cl_subset_coe_cl X), 
 end 
 
-lemma flat_iff_carrier {F : set α} : 
-  M.flat F ↔ M.carrier.flat (F ∪ M.Eᶜ) ∧ F ⊆ M.E :=
+lemma subset_cl_iff_cl_subset_cl (hX : X ⊆ M.E) : X ⊆ M.cl Y ↔ M.cl X ⊆ M.cl Y :=
+⟨λ h, inter_subset_inter (matroid.cl_subset_cl_of_subset_cl (h.trans (M.cl_subset_coe_cl _))) 
+  subset.rfl, λ h, subset_trans (subset_cl hX) h⟩
+
+lemma flat.subset_ground (hF : M.flat F) : F ⊆ M.E := hF.2 
+
+lemma flat.cl (hF : M.flat F) : M.cl F = F := 
 begin
+  refine (subset_cl hF.subset_ground).antisymm' _,
+  convert inter_subset_inter_left M.E hF.1.cl.subset using 1, 
+  { convert rfl using 2,
+    rw [←cl_union_cl_right_eq_cl_union, cl_eq_loops_of_subset (compl_ground_subset_loops_coe _), 
+      cl_union_cl_right_eq_cl_union, union_empty], 
+    apply_instance },
+  rw [inter_distrib_right, inter_eq_left_iff_subset.mpr hF.subset_ground, compl_inter_self, 
+    union_empty], 
+end 
+
+lemma loop.mem_ground (he : M.loop e) : e ∈ M.E := he.2 
+
+lemma loop.dep (he : M.loop e) : ¬ M.indep {e} := matroid.loop.dep he.1 
+
+lemma loop_iff_dep (he : e ∈ M.E) : M.loop e ↔ ¬ M.indep {e} := 
+⟨loop.dep, λ h, ⟨matroid.loop_iff_dep.mpr h, he⟩⟩ 
+
+lemma loop_iff_mem_cl_empty : M.loop e ↔ e ∈ M.cl ∅ := iff.rfl 
+
+lemma nonloop_iff_coe (e : α) : M.nonloop e ↔ (M : matroid α).nonloop e := iff.rfl 
+
+lemma nonloop.indep (he : M.nonloop e) : M.indep {e} := matroid.nonloop.indep he 
+
+lemma nonloop_iff_indep : M.nonloop e ↔ M.indep {e} := matroid.nonloop_iff_indep 
+
+lemma nonloop.mem_ground (he : M.nonloop e) : e ∈ M.E := 
+singleton_subset_iff.mp he.indep.subset_ground 
+
+lemma r_eq_coe_r (X : set α) : M.r X = (M : matroid α).r X := rfl 
+
+lemma r_compl_ground : M.r M.Eᶜ = 0 := 
+r_eq_zero_iff_subset_loops.mpr (compl_ground_subset_loops_coe _)
+
+lemma coe_r_compl_ground (M : matroid_in α) : (M : matroid α).r M.Eᶜ = 0 := r_compl_ground
   
-end 
+lemma r_eq_r_inter_ground (X : set α): 
+  M.r X = M.r (X ∩ M.E) := 
+by rw [←compl_compl M.E, inter_comm, ←diff_eq_compl_inter, r_eq_coe_r, r_eq_coe_r, 
+    ←matroid.r_eq_r_diff_r_zero _ M.coe_r_compl_ground] 
 
--- lemma cl_eq_carrier_cl_inter_ground (M : matroid_in α) (X : set α) : 
---   M.cl X = M.carrier.cl X ∩ M.E :=
+lemma cocircuit_iff_coe (K : set α) : M.cocircuit K ↔ (M : matroid α).cocircuit K := iff.rfl 
+
+lemma cocircuit.subset_ground (hK : M.cocircuit K) : K ⊆ M.E := 
+λ x hx, matroid_in.nonloop.mem_ground (hK.nonloop_of_mem hx)
+
+lemma hyperplane.subset_ground (hF : M.hyperplane F) : F ⊆ M.E := hF.2
+
+-- TODO : hyperplanes, flats, cl definitions are equivalent to the usual ones. 
+
+lemma eq_of_coe_eq_coe {M₁ M₂ : matroid_in α} (h : M₁.E = M₂.E) (h' : (M₁ : matroid α) = M₂) :
+  M₁ = M₂ := 
+by { ext, rw h, simp_rw [carrier_eq_coe, h'] }
+
+lemma eq_of_base_iff_base {M₁ M₂ : matroid_in α} (h : M₁.E = M₂.E) 
+(h' : ∀ B, M₁.base B ↔ M₂.base B) : M₁ = M₂ :=
+by {apply matroid_in.ext, assumption, ext B, exact h' B}
+
+end basic
+
+
+
+variables {M₁ M₂ M : matroid_in α} {X Y I B C : set α} {e f x y : α}
+
+-- section carrier
+
+-- /- The lemmas in this section break the abstraction between `M` and its `carrier`, and are only
+--   used for basic API setup. -/
+
+-- lemma subset_ground_of_disjoint_loops (hX : disjoint X (M.carrier.cl ∅)) : 
+--   X ⊆ M.E :=
+-- (subset_compl_iff_disjoint_right.mpr hX).trans (compl_subset_comm.mp M.support) 
+
+-- lemma mem_ground_of_nonloop (he : ¬M.carrier.loop e) : 
+--   e ∈ M.E :=
 -- begin
---   rw [cl, flat], 
+--   rw [loop_iff_mem_cl_empty] at he,
+--   by_contra h',
+--   rw ←mem_compl_iff at h',
+--   exact he (M.support h')
+-- end
+
+-- lemma subset_ground_of_base_carrier (hB : M.carrier.base B) : 
+--   B ⊆ M.E := 
+-- λ e he, mem_ground_of_nonloop (hB.indep.nonloop_of_mem he)  
+
+-- lemma subset_ground_of_indep_carrier (hI : M.carrier.indep I) : 
+--   I ⊆ M.E :=
+-- by {obtain ⟨B, hB, hIB⟩ := hI, exact hIB.trans (subset_ground_of_base_carrier hB)}
+
+-- lemma indep_iff_carrier_indep :
+--   M.indep I ↔ M.carrier.indep I :=
+-- by simp_rw [matroid_in.indep, matroid_in.base, matroid.indep_iff_subset_base]
+
+-- lemma r_ground_compl (M : matroid_in α) :
+--   M.r (M.Eᶜ) = 0 :=
+-- begin
+--   refine r_eq_zero_of_loopy (λ e he, by_contra (λ he', he (mem_ground_of_nonloop _))), 
+--   rwa loop_iff_r, 
 -- end 
 
+-- lemma flat_iff_carrier {F : set α} : 
+--   M.flat F ↔ M.carrier.flat (F ∪ M.Eᶜ) ∧ F ⊆ M.E :=
+-- begin
+  
+-- end 
 
-end carrier
+-- -- lemma cl_eq_carrier_cl_inter_ground (M : matroid_in α) (X : set α) : 
+-- --   M.cl X = M.carrier.cl X ∩ M.E :=
+-- -- begin
+-- --   rw [cl, flat], 
+-- -- end 
 
-lemma base.indep (hB : M.base B) :
-  M.indep B :=
-⟨B, hB, subset.rfl⟩
 
-lemma indep.subset_E (hI : M.indep I) : 
-  I ⊆ M.E := 
-let ⟨B,hB,hIB⟩ := hI in hIB.trans (subset_ground_of_base_carrier hB)
+-- end carrier
 
-lemma r_le_r_of_subset (M : matroid_in α) (hXY : X ⊆ Y) :
-  M.r X ≤ M.r Y :=
-M.carrier.r_mono hXY
+-- lemma base.indep (hB : M.base B) :
+--   M.indep B :=
+-- ⟨B, hB, subset.rfl⟩
 
-lemma indep.r (hI : M.indep I) :
-  M.r I = I.ncard :=
-by rw [matroid_in.r, (indep_iff_carrier_indep.mp hI).r]
+-- lemma indep.subset_E (hI : M.indep I) : 
+--   I ⊆ M.E := 
+-- let ⟨B,hB,hIB⟩ := hI in hIB.trans (subset_ground_of_base_carrier hB)
 
-lemma empty_indep (M : matroid_in α) :
-  M.indep ∅ :=
-M.carrier.empty_indep
+-- lemma r_le_r_of_subset (M : matroid_in α) (hXY : X ⊆ Y) :
+--   M.r X ≤ M.r Y :=
+-- M.carrier.r_mono hXY
 
-lemma indep.subset_basis_of_subset (hI : M.indep I) (hX : I ⊆ X) :
-  ∃ J, M.basis J X ∧ I ⊆ J :=
-begin
-  obtain ⟨J,hIJ,hJ⟩ := (indep_iff_carrier_indep.mp hI).subset_basis_of_subset hX,
-  refine ⟨J,⟨hJ.indep,hJ.subset,λ J' hJ' hJJ' hJ'X, _⟩,hIJ⟩,
-  exact hJ.eq_of_subset_indep hJ' hJJ' hJ'X,
-end
+-- lemma indep.r (hI : M.indep I) :
+--   M.r I = I.ncard :=
+-- by rw [matroid_in.r, (indep_iff_carrier_indep.mp hI).r]
 
-lemma exists_basis (M : matroid_in α) (X : set α) :
-  ∃ I, M.basis I X :=
-let ⟨I, hIX, h⟩ := M.empty_indep.subset_basis_of_subset (empty_subset X) in ⟨I,hIX⟩
+-- lemma empty_indep (M : matroid_in α) :
+--   M.indep ∅ :=
+-- M.carrier.empty_indep
 
-lemma basis.r (hI : M.basis I X) :
-  M.r I = M.r X :=
-@matroid.basis.r _ _ M.carrier _ _ hI
+-- lemma indep.subset_basis_of_subset (hI : M.indep I) (hX : I ⊆ X) :
+--   ∃ J, M.basis J X ∧ I ⊆ J :=
+-- begin
+--   obtain ⟨J,hIJ,hJ⟩ := (indep_iff_carrier_indep.mp hI).subset_basis_of_subset hX,
+--   refine ⟨J,⟨hJ.indep,hJ.subset,λ J' hJ' hJJ' hJ'X, _⟩,hIJ⟩,
+--   exact hJ.eq_of_subset_indep hJ' hJJ' hJ'X,
+-- -- end
 
-lemma basis.indep (hI : M.basis I X) :
-  M.indep I :=
-@matroid.basis.indep _ _ M.carrier _ _ hI
+-- lemma exists_basis (M : matroid_in α) (X : set α) :
+--   ∃ I, M.basis I X :=
+-- let ⟨I, hIX, h⟩ := M.empty_indep.subset_basis_of_subset (empty_subset X) in ⟨I,hIX⟩
 
-lemma r_eq_r_inter_E (X : set α): 
-  M.r X = M.r (X ∩ M.E) := 
-begin
-  rw [matroid_in.r, ←compl_compl M.E, inter_comm, ←diff_eq_compl_inter, 
-    ←r_eq_r_diff_r_zero X M.r_ground_compl], 
-  refl, 
-end 
 
-lemma eq_of_base_iff_base {M₁ M₂ : matroid_in E} (h : M₁.E = M₂.E) 
-(h' : ∀ B, M₁.base B ↔ M₂.base B) : 
-  M₁ = M₂ :=
-by {apply matroid_in.ext, assumption, ext B, exact h' B}
 
 section equivalence 
 
 /-- A `matroid_in` gives a matroid on a subtype -/
 def to_matroid_of_ground_eq (M : matroid_in α) (hX : M.E = X) : 
   matroid X :=
-{ base := M.carrier.base ∘ (set.image coe),
+{ base := (M : matroid α).base ∘ (set.image coe),
   exists_base' := begin
-    obtain ⟨B,hB⟩ := M.carrier.exists_base',
-    refine ⟨coe ⁻¹' B, _⟩, simp only [function.comp_app, subtype.image_preimage_coe],
-    convert hB,
-    rw [inter_eq_left_iff_subset, ←hX],
-    apply matroid_in.subset_ground_of_disjoint_loops,
-    exact hB.indep.disjoint_loops,
+    obtain ⟨B,hB⟩ := M.exists_base,
+    refine ⟨coe ⁻¹' B, _⟩, 
+    rwa [function.comp_app, subtype.image_preimage_coe, ←matroid_in.base, ←hX, 
+      inter_eq_left_iff_subset.mpr hB.subset_ground],
   end,
   base_exchange' := begin
     subst hX,
     rintro B₁ B₂ hB₁ hB₂ a ha,
-    simp only [function.comp_app] at hB₁ hB₂,
+    simp only [function.comp_app] at hB₁ hB₂ ⊢,
+
     have ha' : (a : α) ∈ (coe '' B₁) \ (coe '' B₂),
     { rw [←image_diff (subtype.coe_injective), mem_image], exact ⟨a,ha,rfl⟩},
     obtain ⟨y,hy,hy'⟩ :=  hB₁.exchange hB₂ ha',
-    refine ⟨⟨y, _⟩, _, _⟩,
-    { exact mem_ground_of_nonloop (hB₂.indep.nonloop_of_mem hy.1), },
+    refine ⟨⟨y, mem_ground_of_nonloop_coe (hB₂.indep.nonloop_of_mem hy.1)⟩, _, _⟩,
     { simp only [←image_diff (subtype.coe_injective), mem_image,
         subtype.exists, subtype.coe_mk, exists_and_distrib_right, exists_eq_right] at hy,
       obtain ⟨hy'',h_eq⟩ := hy,
       exact h_eq},
-    rwa [function.comp_app, image_insert_eq, image_diff subtype.coe_injective, image_singleton],
+    rwa [image_insert_eq, image_diff subtype.coe_injective, image_singleton],
   end }
 
 def to_matroid (M : matroid_in α) : matroid (M.E) := M.to_matroid_of_ground_eq rfl 
@@ -241,8 +362,8 @@ def of_matroid_in {E : set α} (M : matroid E) :
     end },
   support :=
   (begin
-    rintro e (he : e ∉ E), 
-    rw [←loop_iff_mem_cl_empty, loop_iff_not_mem_base_forall],  
+    rintro e he,  
+    rw [←matroid.loop_iff_mem_cl_empty, matroid.loop_iff_not_mem_base_forall],
     rintro B ⟨-,hB⟩ heB, 
     exact he (hB heB), 
   end) }
@@ -257,20 +378,22 @@ def matroid_in_equiv_subtype {E : set α} :
     subst hM, 
     ext, refl, 
     simp only [function.comp_app, subtype.image_preimage_coe, of_matroid_in, 
-      to_matroid_of_ground_eq, subtype.coe_mk], 
+      to_matroid_of_ground_eq, subtype.coe_mk, carrier_eq_coe, ←base_iff_coe ], 
     split, 
     { rintro ⟨hB, hBG⟩, convert hB, rwa [eq_comm, inter_eq_left_iff_subset]},
     intro hB,
-    rw [inter_eq_left_iff_subset.mpr (subset_ground_of_base_carrier hB)],
-    exact ⟨hB, subset_ground_of_base_carrier hB⟩,
+    rw [inter_eq_left_iff_subset.mpr hB.subset_ground],
+    exact ⟨hB, hB.subset_ground⟩,
   end,
   right_inv := begin
     rintro M, 
     ext B, 
-    simp only [of_matroid_in, function.comp_app, image_subset_iff, to_matroid_of_ground_eq, 
-      subtype.coe_preimage_self, subset_univ, and_true], 
-    rw preimage_image_eq _ (subtype.coe_injective), 
+    simp only [of_matroid_in, to_matroid_of_ground_eq, ←carrier_eq_coe, function.comp_app, 
+      image_subset_iff, subtype.coe_preimage_self, subset_univ, and_true, 
+      preimage_image_eq _ (subtype.coe_injective)], 
   end }
+
+
 
 
 @[simp] lemma matroid_in_equiv_subtype_apply_base {E : set α} {B : set E} 
@@ -281,9 +404,11 @@ by simp only [matroid_in_equiv_subtype, to_matroid_of_ground_eq, matroid_in.base
 
 @[simp] lemma matroid_in_equiv_subtype_apply_symm_base {B E : set α} (M : matroid E) :
   (matroid_in_equiv_subtype.symm M : matroid_in α).base B ↔ M.base (coe ⁻¹' B) ∧ B ⊆ E :=
-by simp only [matroid_in_equiv_subtype, of_matroid_in, matroid_in.base,
-    equiv.coe_fn_symm_mk, subtype.coe_mk]
- 
+by { rw [matroid_in_equiv_subtype, equiv.coe_fn_symm_mk, subtype.coe_mk, of_matroid_in ], refl } 
+
+end equivalence
+
+/-
 @[simp] lemma matroid_in_equiv_subtype_apply_indep {E : set α} {I : set E} 
 (M : {M : matroid_in α // M.E = E}) :
   (matroid_in_equiv_subtype M).indep I ↔ (M : matroid_in α).indep (coe '' I) := 
@@ -356,6 +481,9 @@ lemma eq_coe_image_preimage {E : set α} (M : matroid_in α) (h : M.E = E):
   M = matroid_in_equiv_subtype.symm (matroid_in_equiv_subtype ⟨M, h⟩) := 
 by simp only [equiv.symm_apply_apply, subtype.coe_mk]
 
+-/
+
+/-
 end equivalence 
 
 section ext
@@ -382,7 +510,10 @@ end
 
 
 
+
 end ext 
+
+-/
 
 section dual
 
@@ -390,13 +521,15 @@ section dual
 def dual (M : matroid_in α) : matroid_in α :=
   matroid_in_equiv_subtype.symm (matroid_in_equiv_subtype ⟨M, rfl⟩).dual
 
+-- def dual (M : matroid_in α)
+
 reserve postfix `*` :90 
 
 notation (name := matroid_in_dual) M* := matroid_in.dual M 
 
 lemma dual_base_iff : 
   M*.base B ↔ M.base (M.E \ B) ∧ B ⊆ M.E :=
-by simp [dual, image_compl_preimage]
+by { simp [dual, image_compl_preimage], }
 
 @[simp] lemma dual_E (M : matroid_in α): 
   M*.E = M.E := 
@@ -411,7 +544,7 @@ begin
   split, 
   { rintro ⟨⟨h, -⟩, hB⟩, rwa [inter_eq_right_iff_subset.mpr hB] at h},
   intro hB, 
-  have h := hB.indep.subset_E, 
+  have h := hB.indep.subset_ground, 
   exact ⟨⟨by rwa inter_eq_right_iff_subset.mpr h, diff_subset _ _⟩, h⟩, 
 end 
 
